Concede stylistic minutiae

theories/Hole.v
@@ -7,22 +7,22 @@ From LambdaST Require Import
 
 Inductive hole : Set :=
   | HoleHere
-  | HoleCommaL (lhs : hole) (rhs : context)
-  | HoleCommaR (lhs : context) (rhs : hole)
-  | HoleSemicL (lhs : hole) (rhs : context)
-  | HoleSemicR (lhs : context) (rhs : hole)
+  | HoleCommaL (h : hole) (g : context)
+  | HoleCommaR (g : context) (h : hole)
+  | HoleSemicL (h : hole) (g : context)
+  | HoleSemicR (g : context) (h : hole)
   .
 Hint Constructors hole : core.
 Derive Show for hole.
 Derive Arbitrary for hole.
 
-Fixpoint fill h y :=
+Fixpoint fill h D :=
   match h with
-  | HoleHere => y
-  | HoleCommaL lhs rhs => CtxComma (fill lhs y) rhs
-  | HoleCommaR lhs rhs => CtxComma lhs (fill rhs y)
-  | HoleSemicL lhs rhs => CtxSemic (fill lhs y) rhs
-  | HoleSemicR lhs rhs => CtxSemic lhs (fill rhs y)
+  | HoleHere => D
+  | HoleCommaL lhs rhs => CtxComma (fill lhs D) rhs
+  | HoleCommaR lhs rhs => CtxComma lhs (fill rhs D)
+  | HoleSemicL lhs rhs => CtxSemic (fill lhs D) rhs
+  | HoleSemicR lhs rhs => CtxSemic lhs (fill rhs D)
   end.
 
 Inductive Fill : hole -> context -> context -> Prop :=
@@ -77,6 +77,11 @@ Lemma fv_fill : forall h plug ctx,
 Proof. intros. induction H; sfirstorder. Qed.
 Hint Resolve fv_fill : core.
 
+Lemma fv_fill_fn : forall h plug,
+  SetEq (fv_ctx (fill h plug)) (set_union (fv plug) (fv h)).
+Proof. intros. remember (fill h plug) as ctx eqn:E. apply reflect_fill in E. apply fv_fill. assumption. Qed.
+Hint Resolve fv_fill_fn : core.
+
 Inductive WFHole : hole -> Prop :=
   | WFHoleHere :
       WFHole HoleHere
@@ -102,17 +107,6 @@ Inductive WFHole : hole -> Prop :=
       WFHole (HoleSemicR g h)
   .
 Hint Constructors WFHole : core.
-
-Theorem wf_ctx_plug : forall GD,
-  WFContext GD ->
-  forall G D,
-  Fill G D GD ->
-  WFContext D.
-Proof.
-  intros GD Hc G D Hf. generalize dependent Hc.
-  induction Hf; intros; try (apply IHHf; sinvert Hc); assumption.
-Qed.
-Hint Resolve wf_ctx_plug : core.
 
 Theorem fill_disjoint_l : forall G D GD (s : context),
   Fill G D GD ->
@@ -146,7 +140,18 @@ Proof.
 Qed.
 Hint Resolve wf_ctx_hole : core.
 
-Lemma wf_fill : forall G D GD,
+Theorem wf_ctx_plug : forall GD,
+  WFContext GD ->
+  forall G D,
+  Fill G D GD ->
+  WFContext D.
+Proof.
+  intros GD Hc G D Hf. generalize dependent Hc.
+  induction Hf; intros; try (apply IHHf; sinvert Hc); assumption.
+Qed.
+Hint Resolve wf_ctx_plug : core.
+
+Lemma wf_ctx_fill : forall G D GD,
   Fill G D GD ->
   WFHole G ->
   WFContext D ->
@@ -158,7 +163,7 @@ Proof.
   constructor; try assumption (* 1/3 *); try eapply IHHG; clear IHHG; try eassumption;
   apply fv_fill in H5; (* <-- this is the crucial move! *) sfirstorder.
 Qed.
-Hint Resolve wf_fill : core.
+Hint Resolve wf_ctx_fill : core.
 
 Lemma fill_wf_disjoint : forall G D GD,
   Fill G D GD ->
@@ -178,9 +183,20 @@ Theorem wf_hole_iff : forall G D GD,
     WFContext GD <-> (
       WFHole G /\
       WFContext D /\
-      DisjointSets (fv G) (fv D))). (* <-- this should fix the above comment *)
+      DisjointSets (fv G) (fv D))).
 Proof.
   intros G D GD Hf. split; [intro Hwf | intros [HG [HD Hd]]].
   - split; [| split]; [eapply wf_ctx_hole | eapply wf_ctx_plug | eapply fill_wf_disjoint]; eassumption.
-  - eapply wf_fill; eassumption.
+  - eapply wf_ctx_fill; eassumption.
 Qed.
+Hint Resolve wf_hole_iff : core.
+
+Theorem wf_fill : forall h d,
+  WFContext (fill h d) <-> (WFHole h /\ WFContext d /\ DisjointSets (fv h) (fv d)).
+Proof.
+  intros h d.
+  remember (fill h d) as g.
+  apply reflect_fill in Heqg.
+  hauto l: on use: wf_hole_iff.
+Qed.
+Hint Resolve wf_fill : core.
