theories/Typing.v
@@ -21,10 +21,6 @@ Inductive Typed : context -> term -> type -> Prop :=
       x <> y ->
       ~fv G x ->
       ~fv G y ->
-      (*
-      fill G (CtxComma (CtxHasTy x s) (CtxHasTy y t)) |- e \in r ->
-      fill G (CtxHasTy z (TyPar s t)) |- (TmLetPar x y z e) \in r
-      *)
       Fill G (CtxComma (CtxHasTy x s) (CtxHasTy y t)) Gxsyt ->
       Fill G (CtxHasTy z (TyPar s t)) Gzst ->
       Gxsyt |- e \in r ->
@@ -38,10 +34,6 @@ Inductive Typed : context -> term -> type -> Prop :=
       x <> y ->
       ~fv G x ->
       ~fv G y ->
-      (*
-      fill G (CtxSemic (CtxHasTy x s) (CtxHasTy y t)) |- e \in r ->
-      fill G (CtxHasTy z (TyDot s t)) |- (TmLetCat t x y z e) \in r
-      *)
       Fill G (CtxSemic (CtxHasTy x s) (CtxHasTy y t)) Gxsyt ->
       Fill G (CtxHasTy z (TyDot s t)) Gzst ->
       Gxsyt |- e \in r ->
@@ -51,7 +43,6 @@ Inductive Typed : context -> term -> type -> Prop :=
   | TOneR : forall G,
       G |- unit \in 1
   | TVar : forall G x s Gxs,
-      (* fill G (CtxHasTy x s) |- (TmVar x) \in s *)
       Fill G (CtxHasTy x s) Gxs ->
       Gxs |- TmVar x \in s
   | TSubCtx : forall G G' e s,
@@ -61,19 +52,11 @@ Inductive Typed : context -> term -> type -> Prop :=
   | TLet : forall G D x e e' s t Gxs GD,
       ~fv G x ->
       D |- e \in s ->
-      (*
-      fill G (CtxHasTy x s) |- e' \in t ->
-      fill G D |- TmLet x e e' \in t
-      *)
       Fill G (CtxHasTy x s) Gxs ->
       Fill G D GD ->
       Gxs |- e' \in t ->
       GD |- TmLet x e e' \in t
   | TDrop : forall G x s t e Ge Gxs,
-      (*
-      fill G CtxEmpty |- e \in t ->
-      fill G (CtxHasTy x s) |- TmDrop x e \in t
-      *)
       Fill G CtxEmpty Ge ->
       Fill G (CtxHasTy x s) Gxs ->
       Ge |- e \in t ->
@@ -111,6 +94,7 @@ Hint Resolve typed_fv : core.
 
 (* TODO: add WF weakening theorem assuming all FVs are covered, then use the above to prove the below *)
 
+(*
 Theorem typed_wf_term : forall G x T,
   G |- x \in T ->
   WFTerm (fv G) x.
@@ -129,3 +113,4 @@ Proof.
     *)
   - (* (e1; e2) *)
     cbn in *. constructor. eapply typed_fv in H. Abort. (* TODO *)
+*)
